verify basic properties on vec_ty

theories/typing/lib/vec.v
@@ -2,6 +2,7 @@ From lrust.typing Require Export type.
 From lrust.typing Require Import array_util typing.
 
 Open Scope nat.
+Implicit Type 𝔄 𝔅: syn_type.
 
 Notation "l ↦∗len n" := (∃vl, ⌜length vl = n%nat⌝ ∗ l ↦∗ vl)%I
   (at level 20, format "l  ↦∗len  n") : bi_scope.
@@ -12,7 +13,7 @@ Section vec.
   Definition freeable_sz' (sz: nat) (l: loc) : iProp Σ :=
     †{1}l…sz ∨ ⌜Z.of_nat sz = 0⌝.
 
-  Program Definition vec {𝔄} (ty: type 𝔄) : type (listₛ 𝔄) := {|
+  Program Definition vec_ty {𝔄} (ty: type 𝔄) : type (listₛ 𝔄) := {|
     ty_size := 3;  ty_lfts := ty.(ty_lfts);  ty_E := ty.(ty_E);
     ty_own alπ d tid vl :=
       [S(d') := d] ∃(len ex: nat) (l: loc) (aπl: vec (proph 𝔄) len),
@@ -80,14 +81,63 @@ Section vec.
     iExists _, _, _, _. by iFrame.
   Qed.
 
-  Global Instance vec_ne {𝔄} : NonExpansive (@vec 𝔄).
+  Global Instance vec_ty_ne {𝔄} : NonExpansive (@vec_ty 𝔄).
   Proof. solve_ne_type. Qed.
 
-  Global Instance vec_type_contractive 𝔄 : TypeContractive (@vec 𝔄).
+  Global Instance vec_type_contractive 𝔄 : TypeContractive (@vec_ty 𝔄).
   Proof.
     split; [by apply type_lft_morphism_id_like|done| |].
     - move=>/= > ->*. do 19 (f_contractive || f_equiv). by simpl in *.
     - move=>/= > ->*. do 16 (f_contractive || f_equiv). by simpl in *.
   Qed.
 
+  Global Instance vec_send {𝔄} (ty: type 𝔄) : Send ty → Send (vec_ty ty).
+  Proof. move=> ?>/=. by do 19 f_equiv. Qed.
+
+  Global Instance vec_sync {𝔄} (ty: type 𝔄) : Sync ty → Sync (vec_ty ty).
+  Proof. move=> ?>/=. by do 16 f_equiv. Qed.
+
+  Lemma vec_leak {𝔄} (ty: type 𝔄) Φ E L :
+    leak E L ty Φ → leak E L (vec_ty ty) (lforall Φ).
+  Proof.
+    iIntros (Lk ? q ?[|]???) "#LFT #PROPH #E L vec //=".
+    iDestruct "vec" as (?? l aπl[->->]) "[↦tys _]". iIntros "!>!>!>".
+    iInduction aπl as [|] "IH" forall (q l)=>/=.
+    { iApply step_fupdN_full_intro. iFrame. by iApply proph_obs_true. }
+    iDestruct "↦tys" as "[(%&_& ty) ↦tys]". iDestruct "L" as "[L L₊]".
+    iMod (Lk with "LFT PROPH E L ty") as "Upd"; [done|].
+    setoid_rewrite <-shift_loc_assoc_nat. iMod ("IH" with "L₊ ↦tys") as "Upd'".
+    iCombine "Upd Upd'" as "Upd". iApply (step_fupdN_wand with "Upd").
+    iIntros "!>[>[#? $] >[#? $]]". by iApply proph_obs_and.
+  Qed.
+
+  Lemma vec_leak_just {𝔄} (ty: type 𝔄) E L :
+    leak E L ty (const True) → leak E L (vec_ty ty) (const True).
+  Proof. move=> ?. apply leak_just. Qed.
+
+  Lemma vec_subtype {𝔄 𝔅} (f: 𝔄 → 𝔅) ty ty' E L :
+    subtype E L ty ty' f → subtype E L (vec_ty ty) (vec_ty ty') (map f).
+  Proof.
+    iIntros (Sub ?) "L". iDestruct (Sub with "L") as "#Sub". iIntros "!> E".
+    iDestruct ("Sub" with "E") as "(%EqSz & #? & #InOwn & #InShr)".
+    have Eq: ∀(aπl: vec (proph 𝔄) _), map f ∘ lapply aπl = lapply (vmap (f ∘.) aπl).
+    { move=> ?. elim; [done|]=> ??? IH. fun_ext=>/= ?. f_equal. apply (equal_f IH). }
+    do 2 (iSplit; [done|]). iSplit; iIntros "!>" (?[|]) "* vec //=".
+    - iDestruct "vec" as (?? l aπl [->->]) "(↦tys & ex & †)".
+      iExists _, _, _, _. rewrite Eq EqSz. iSplit; [done|]. iFrame "ex †".
+      iNext. iInduction aπl as [|] "IH" forall (l)=>/=; [done|].
+      iDestruct "↦tys" as "[(%& ↦ & ty) ↦tys]". setoid_rewrite <-shift_loc_assoc_nat.
+      iDestruct ("IH" with "↦tys") as "$". iExists _. iFrame "↦". by iApply "InOwn".
+    - iDestruct "vec" as (?? l' ?->) "(↦ & tys)". iExists _, _, _, _.
+      rewrite Eq EqSz. iSplit; [done|]. iFrame "↦". iNext.
+      iInduction aπl as [|] "IH" forall (l')=>/=; [done|].
+      iDestruct "tys" as "[ty tys]". setoid_rewrite <-shift_loc_assoc_nat.
+      iDestruct ("IH" with "tys") as "$". by iApply "InShr".
+  Qed.
+  Lemma vec_eqtype {𝔄 𝔅} (f: 𝔄 → 𝔅) g ty ty' E L :
+    eqtype E L ty ty' f g → eqtype E L (vec_ty ty) (vec_ty ty') (map f) (map g).
+  Proof. move=> [??]. split; by apply vec_subtype. Qed.
 End vec.
+
+Global Hint Resolve vec_leak | 5 : lrust_typing.
+Global Hint Resolve vec_leak_just vec_subtype vec_eqtype : lrust_typing.
